lean/LeanTs/Decl.lean
@@ -1409,6 +1409,18 @@ theorem compileExpr_types_irrel {p q : Program} (h : q.types = p.types) {e : Exp
     intro ctx
     rw [Compile.compileExpr.eq_def, Compile.compileExpr.eq_def]
     simp only [ihs ctx, ihlo ctx, ihhi ctx]
+  | index _ _ iharr ihidx =>
+    intro ctx
+    rw [Compile.compileExpr.eq_def, Compile.compileExpr.eq_def]
+    simp only [iharr ctx, ihidx ctx]
+  | arraySlice _ _ _ iharr ihlo ihhi =>
+    intro ctx
+    rw [Compile.compileExpr.eq_def, Compile.compileExpr.eq_def]
+    simp only [iharr ctx, ihlo ctx, ihhi ctx]
+  | arrayReverse _ iharr =>
+    intro ctx
+    rw [Compile.compileExpr.eq_def, Compile.compileExpr.eq_def]
+    simp only [iharr ctx]
 
 theorem compileFinish_types_irrel {p q : Program} (h : q.types = p.types) {e : Expr}
     (hfrag : InFragment e) (ctx : Ctx) (acc : List Js.Stmt) :
